\subsection*{Task 2.1}

\subsubsection*{Task 2.1.1}

We've got three homogeneous transformations each with a rotation $R_i$ around the z-Axis and a translation $a_i$.

\begin{align*}
^0A_1 &= 
\begin{pmatrix}
C_1 & -S_1 & 0 & C_1a_1 \\
S_1 & C_1 & 0 & S_1a_1 \\
0 & 0 & 1 & 0 \\
0 & 0 & 0 & 1 
\end{pmatrix},
\,^1A_2 = 
\begin{pmatrix}
C_2 & -S_2 & 0 & C_2a_2 \\
S_2 & C_2 & 0 & S_2a_2 \\
0 & 0 & 1 & 0 \\
0 & 0 & 0 & 1 
\end{pmatrix} \\
^2A_3 &= 
\begin{pmatrix}
C_3 & -S_3 & 0 & C_3a_3 \\
S_3 & C_3 & 0 & S_3a_3 \\
0 & 0 & 1 & 0 \\
0 & 0 & 0 & 1 
\end{pmatrix}
=
\begin{pmatrix}
C(180\degree-\theta_1-\theta_2) & -S(180\degree-\theta_1-\theta_2) & 0 & C(180\degree-\theta_1-\theta_2)a_3 \\
S(180\degree-\theta_1-\theta_2) & C(180\degree-\theta_1-\theta_2) & 0 & S(180\degree-\theta_1-\theta_2)a_3 \\
0 & 0 & 1 & 0 \\
0 & 0 & 0 & 1 
\end{pmatrix} \\
&\text{with } S(180\degree-\alpha) = S(\alpha), C(180\degree-\alpha) = -C(\alpha)\\
& \text{and } C_{12} = C(\theta_1+\theta_2) = -C(180\degree-\theta_1-\theta_2) = -C_3,\\
& S_{12} = S(\theta_1+\theta_2) = S(180\degree-\theta_1-\theta_2) = S_3\\
&=
\begin{pmatrix}
-C_{12} & -S_{12} & 0 & -C_{12}a_3 \\
S_{12} & -C_{12} & 0 & S_{12}a_3 \\
0 & 0 & 1 & 0 \\
0 & 0 & 0 & 1 
\end{pmatrix}
=
\begin{pmatrix}
-C_1C_2+S_1S_2 & -S_1C_2-C_1S_2 & 0 & (-C_1C_2+S_1S_2)a_3 \\
S_1C_2+C_1S_2 & -C_1C_2+S_1S_2 & 0 & (S_1C_2+C_1S_2)a_3 \\
0 & 0 & 1 & 0 \\
0 & 0 & 0 & 1 
\end{pmatrix} \\
^0T_3 &= \,^0A_1\cdot\,^1A_2\cdot\,^2A_3 =
\begin{pmatrix}
C_1 & -S_1 & 0 & C_1a_1 \\
S_1 & C_1 & 0 & S_1a_1 \\
0 & 0 & 1 & 0 \\
0 & 0 & 0 & 1 
\end{pmatrix}\cdot
\begin{pmatrix}
C_2 & -S_2 & 0 & C_2a_2 \\
S_2 & C_2 & 0 & S_2a_2 \\
0 & 0 & 1 & 0 \\
0 & 0 & 0 & 1 
\end{pmatrix}\cdot
\begin{pmatrix}
-C_{12} & -S_{12} & 0 & -C_{12}a_3 \\
S_{12} & -C_{12} & 0 & S_{12}a_3 \\
0 & 0 & 1 & 0 \\
0 & 0 & 0 & 1 
\end{pmatrix}\\
&= 
\begin{pmatrix}
C_1C_2-S_1S_2 & -C_1S_2-S_1C_2 & 0 & C_1C_2a_2-S_1S_2a_2+C_1a_1 \\
S_1C_2+C_1S_2 & -S_1S_2+C_1C_2 & 0 & S_1C_2a_2+C_1S_2a_2+S_1a_1 \\
0 & 0 & 1 & 0 \\
0 & 0 & 0 & 1 
\end{pmatrix}\cdot
\begin{pmatrix}
-C_{12} & -S_{12} & 0 & -C_{12}a_3 \\
S_{12} & -C_{12} & 0 & S_{12}a_3 \\
0 & 0 & 1 & 0 \\
0 & 0 & 0 & 1 
\end{pmatrix}\\
&= 
\begin{pmatrix}
C_{12} & -S_{12} & 0 & C_{12}a_2+C_1a_1 \\
S_{12} & C_{12} & 0 & S_{12}a_2+S_1a_1 \\
0 & 0 & 1 & 0 \\
0 & 0 & 0 & 1 
\end{pmatrix}\cdot
\begin{pmatrix}
-C_{12} & -S_{12} & 0 & -C_{12}a_3 \\
S_{12} & -C_{12} & 0 & S_{12}a_3 \\
0 & 0 & 1 & 0 \\
0 & 0 & 0 & 1 
\end{pmatrix}\\
&= 
\begin{pmatrix}
-C_{12}C_{12}-S_{12}S_{12} & -C_{12}S_{12}+S_{12}C_{12} & 0 & (-C_{12}C_{12}-S_{12}S_{12})a_3+C_{12}a_2+C_1a_1 \\
-S_{12}C_{12}+C_{12}S_{12} & -S_{12}S_{12}-C_{12}C_{12} & 0 & (-S_{12}C_{12}+C_{12}S_{12})a_3+S_{12}a_2+S_1a_1 \\
0 & 0 & 1 & 0 \\
0 & 0 & 0 & 1 
\end{pmatrix}
\end{align*}
Using the following equations
\begin{align*}
-C_{12}C_{12}-S_{12}S_{12} &= C(180\degree-(\theta_1+\theta_2))C(\theta_1+\theta_2)-S(180\degree-(\theta_1+\theta_2))S(\theta_1+\theta_2)\\
&= C((180\degree-\theta_1-\theta_2)+\theta_1+\theta_2) = C(180\degree) = -1\\
-C_{12}S_{12}+S_{12}C_{12} &= C(180\degree-(\theta_1+\theta_2))S(\theta_1+\theta_2)+S(180\degree-(\theta_1+\theta_2))C(\theta_1+\theta_2)\\
&= S((180\degree-\theta_1-\theta_2)+\theta_1+\theta_2) = S(180\degree) = 0\\
\end{align*}
we get
\begin{align*}
^0T_3
&= 
\begin{pmatrix}
	-1 & 0 & 0 & -a_3+C_{12}a_2+C_1a_1 \\
	0 & -1 & 0 & S_{12}a_2+S_1a_1 \\
	0 & 0 & 1 & 0 \\
	0 & 0 & 0 & 1 
\end{pmatrix}
= 
\begin{pmatrix}
-1 & 0 & 0 & C_1a_1-C_3a_2-a_3 \\
0 & -1 & 0 & S_1a_1+S_3a_2 \\
0 & 0 & 1 & 0 \\
0 & 0 & 0 & 1 
\end{pmatrix}
\end{align*}

\subsubsection*{Task 2.1.2}
\begin{align*}
^{-1}A_0 &= 
\begin{pmatrix}
1 & 0 & 0 & 0 \\
0 & C_0 & -S_0 & 0 \\
0 & S_0 & C_0 & 0 \\
0 & 0 & 0 & 1 
\end{pmatrix},
\,^{3}A_4 =
\begin{pmatrix}
1 & 0 & 0 & 0 \\
0 & C_4 & -S_4 & 0 \\
0 & S_4 & C_4 & 0 \\
0 & 0 & 0 & 1 
\end{pmatrix}
\end{align*}
